\subsection{Danielli: Summer 2011}
\setcounter{exercise}{0}
\setcounter{equation}{0}

\begin{problem}
  Let \(f\in L^1(\bbR)\), and let
  \(\hat f(x)=\int_{\bbR} f(t)\cos(xt)\diff t\).
  \begin{enumerate}[label=(\alph*)]
  \item Prove that \(\hat f(x)\) is continuous for \(x\in\bbR\).
  \item Prove the following \emph{Riemman--Lebesgue lemma}:
    \[
      \lim_{x\to\infty}\hat f(x)=0.
    \]
  \end{enumerate}
  \emph{Hint}: Start by proving the statement for \(f=\indicate_{[a,b]}\).
\end{problem}
\begin{solution}
  For part (a): let \(\varepsilon>0\) be given. Then, since \(\cos(xt)\) is
  continuous there exists \(\delta'>0\) such that \(|x-y|<\delta\) implies
  \[
    |\cos(xt)-\cos(yt)|<\frac{\varepsilon}{\|f\|_1}.
  \]
  Now, let \(\delta=\delta'\). Then we have
  \begin{align*}
    |\hat f(x)-\hat f(y)|
    &=\left|
      \int_\bbR f(t)\cos(xt)\diff t
      -\int_\bbR f(t)\cos(yt)\diff t
      \right|\\
    &\leq\int_\bbR|f(t)||\cos(xt)-\cos(yt)|\diff t\\
    &<\frac{\varepsilon}{\|f\|_1}\int_\bbR|f(t)|\diff t\\
    &=\frac{\varepsilon}{\|f\|_1}\|f\|_1\\
    &=\varepsilon.
  \end{align*}
  Since this can be done for any \(x\in\bbR\), \(\hat f\) is continuous on
  \(\bbR\).

  For part (b): since simple functions are dense in \(L^1(\bbR)\), \(f\)
  there exists a sequence of simple functions \(\{s_n\}\), \(n\in\bbN\),
  such that \(\int_\bbR s_n\to\|f\|_1\). Therefore, it suffices to prove
  the result for characteristic functions. Let \(f=\indicate_{[a,b]}\) and
  consider the limit
  \[
    \lim_{x\to\infty}\hat f(x)=\lim_{x\to\infty}\int_\bbR f(t)\cos(xt)\diff t.
  \]
  Since \(f=\indicate_{[a,b]}\), we have
  \begin{align*}
    \lim_{x\to\infty}\int_\bbR f(t)\cos(xt)\diff t
    &=\lim_{x\to\infty}\int_a^b\cos(xt)\diff t\\
    &=\lim_{x\to\infty}\biggl[\frac{1}{x}(\sin(xa)-\sin(xb))\biggr]\\
    &=\lim_{x\to\infty}\biggl[\frac{\sin(xa)}{x}-\frac{\sin(xb)}{x}\biggr]\\
    &=\biggl[\lim_{x\to\infty}\frac{\sin(xa)}{x}\biggr]
      -\biggl[\lim_{x\to\infty}\frac{\sin(xb)}{x}\biggr]\\
    &=1-1\\
    &=0,
  \end{align*}
  as we set out to show.
\end{solution}

\begin{problem}
  \hfill
  \begin{enumerate}[label=(\alph*)]
  \item Suppose that \(f_k,f\in L^2(E)\), with \(E\) a measurable set, and
    that
    \[
      \label{eq:aug-11:1}
      \tag{\(\bigstar\)}
      \int_E f_kg\too\int_E fg
    \]
    as \(k\to\infty\) for all \(g\in L^2(E)\). If, in addition,
    \(\|f_k\|_2\to\|f\|_2\) show that \(f_k\) converges to \(f\) in
    \(L^2\), i.e., that
    \[
      \int_E|f-f_k|^2\too 0
    \]
    as \(k\to\infty\).
  \item Provide an example of a sequence \(f_k\) in \(L^2\) and a function
    \(f\) in \(L^2\) satisfying \eqref{eq:aug-11:1}, but such that \(f_k\)
    does \emph{not} converge to \(f\) in \(L^2\).
  \end{enumerate}
\end{problem}
\begin{solution}
  For part (a): expand the limit
  \begin{gather}
    \label{eq:aug-11:2-a}
    \begin{aligned}
      \lim_{n\to\infty}\int_E|f-f_n|^2\diff x
      &=\lim_{n\to\infty}\biggl[\int_E\bigl(|f|^2-2|ff_n|+|f|_n^2\bigr)\diff x\biggr]\\
      &=\lim_{n\to\infty}\biggl[\|f_n\|_2+\|f\|_2-2\int_E f_nf\diff x\biggr]\\
      &=\lim_{n\to\infty}\|f_n\|_2+\lim_{n\to\infty}\|f\|_2-2\lim_{n\to\infty}\int_E
      f_nf\diff x.
    \end{aligned}
  \end{gather}
  Since
  \[
    \int_Ef_ng\diff x\too \int_E fg\diff x
  \]
  for every \(g\in L^p(E)\),
  \[
    \int_E f_nf\diff x\too \int_Ef^2\diff x={\|f\|_2}^{\cramped 2}.
  \]
  Moreover, \(\|f_n\|_2\to\|f\|_2\) so the limit in \eqref{eq:aug-11:2-a}
  converges to
  \[
    \lim_{n\to\infty}\|f_n\|_2+\lim_{n\to\infty}\|f\|_2-2\lim_{n\to\infty}\int_E
    f_nf\diff x
    =%
    \|f\|_2+\|f\|_2-2\|f\|_2=0
  \]
  as \(n\to\infty\).

  For part (b), consider the sequence \(\{f_n\}\), \(n\in\bbN\), where
  \(f_n(x)=\log(n)\exp(-nx)\). Then, we claim that
  \(f_n\xrightarrow{L^2[0,1]}0\), but that \(f_n\nrightarrow 0\)
  pointwise. To see the former, first note that
  \[
    \begin{aligned}
      \lim_{n\to\infty}\biggl[\int_0^1 f_n(x)\diff x\biggr]
      &=\lim_{n\to\infty}\biggl[\int_0^1\log(n)\exp(-nx)\diff x\biggr]\\
      &=\lim_{n\to\infty}\biggl[\log(n)\exp(-nx)\bigr|_0^1\biggr]\\
      &=\lim_{n\to\infty}\biggl[
      \frac{1}{n}\log(n)-\frac{1}{n}\log(n)\exp(-n)
      \biggr]\\
      &=\lim_{n\to\infty}\left[%
        \biggl(\frac{1-\exp(-n)}{n}\biggr)\log(n)%
      \right]\\
      &=0.
    \end{aligned}
  \]
  However, \(f_n\) does not converge to \(0\) a.e.\@ since, for
  \(x=0\) there exist no \(N\in\bbN\) such that
  \[
    |\log(n)|<1.
  \]
  for all \(n\geq N\).
\end{solution}

\begin{problem}
  A bounded function \(f\) is said to be of bounded variation on \(\bbR\)
  if it is of bounded variation on any finite subinterval \([a,b]\), and
  moreover \(A\defeq\sup_{a,b}V[a,b;f]<\infty\). Here, \(V[a,b;f]\) denotes the
  total variation of \(f\) over the interval \([a,b]\). Show that:
\begin{enumerate}[label=(\alph*)]
\item \(\displaystyle\int_{\bbR}|f(x+h)-f(x)|\diff x\leq A|h|\) for all
  \(h\in\bbR\).
  \\\\
  \emph{Hint}: For \(h>0\), write
  \[
    \int_{\bbR} |f(x+h)-f(x)|\diff x=
    \sum_{n=-\infty}^\infty\int_{nh}^{(n+1)h}|f(x+h)-f(x)|\diff x.
  \]
\item
  \(\displaystyle\left|\int_{\bbR} f(x)\varphi'(x)\diff x\right|\leq A\),
  where \(\varphi\) is any function of class \(C^1\), of bounded variation,
  compactly supported, with \(\sup_{x\in\bbR}|\varphi(x)|\leq 1\).
\end{enumerate}
\end{problem}
\begin{solution}
  For part (a), it suffices to consider only positive \(h\) as, making the
  change of variables \(u=x+h\) yields
  \[
    \int_{\bbR} |f(u)-f(u-h)|\diff u=
    \int_{\bbR} |f(u+(-h))-f(u)|\diff u
  \]
  where \(-h\) is positive (and letting \(h=0\), we have a trivial
  inequality). Now, taking the hint, write
  \[
    \int_{\bbR} |f(x+h)-f(x)|\diff x=%
    \sum_{n=-\infty}^\infty\int_{nh}^{(n+1)h}|f(x+h)-f(x)|\diff x.
  \]
  Now, since \(|f((n+1)h)-f(nh)|\) is a sum in the total variation of \(f\)
  on the interval \([nh,(n+1)h]\), \(|f(x+h)-f(x)|\) is bounded by
  \(V[nh,(n+2)h;f]\). Thus, we have
  \begin{align*}
    \int_{\bbR} |f(x+h)-f(x)|\diff x
    &=\sum_{n=-\infty}^\infty\int_{nh}^{(n+1)h}|f(x+h)-f(x)|\diff x\\
    &\leq\sum_{n=-\infty}^\infty\int_{nh}^{(n+1)h}V[nh,(n+2)h;f]\diff x\\
    &=\sum_{n=-\infty}^\infty V[nh,(n+2)h;f]\int_{nh}^{(n+1)h}\diff x\\
    &=\sum_{n=-\infty}^\infty V[nh,(n+2)h;f]|h|\\
    &=2A|h|.
  \end{align*}
  I suspect there is an error here as the most obvious bound we can get is
  \(2A|h|\) and not the stricter \(A|h|\).

  For part (b), \(f\) is absolutely continuous since it is of bounded
  variation and \(\varphi\) is absolutely continuous since it is Lipschitz
  (\(\varphi\) is differentiable on a compact set, thus, by the mean value
  theorem \(|\varphi(x)-\varphi(y)|\leq \varphi'(\xi)|x-y|\) for some
  \(\xi\in\Supp\varphi\)). Assuming \(\Supp\varphi\) has nonempty interior,
  \(\Supp\varphi\) contains a closed interval \(I=[a,b]\) (in fact,
  \(\Supp\varphi\) is of the form \([a,b]\setminus\bigcup_{n\in A} I_n\),
  \(A\subseteq\bbN\), where \(I_n=(a_n,b_n)\) with
  \(a_n,b_n\in\Supp\varphi\)) and thus, by integration by parts, we have
  \begin{align*}
    \int_a^b f\varphi'\diff x%
    &=f(b)\varphi(b)-f(a)\varphi(a)
      -\int_a^b f'\varphi\diff x\\
    &\leq f(b)-f(a)
      -\int_a^b f'\diff x\\
    &=2(f(b)-f(a))\\
    &\leq 2V[a,b;f]
  \end{align*}
  Thus, summing over every
  \[
    \sum_{n=0}^\infty \int_{a_n}^{b_n} f\varphi'\diff x\leq 2|A|.
  \]
\end{solution}

\begin{problem}
  \hfill
  \begin{enumerate}[label=(\alph*)]
  \item Prove the \emph{generalized Hölder's inequality}: Assume
    \(1\leq p_j\leq\infty\), \(j=1,\dotsc,n\), with
    \(\sum_{j=1}^n 1/p_j=1/r\leq 1\). If \(E\) is a measurable set and
    \(f_j\in L^{p_j}(E)\) for \(j=1,\dotsc,n\), then
    \(\prod_{j=1}^n f_j\in L^r(E)\) and
    \[
      \|f_1\dotsm f_n\|_r\leq\|f_1\|_{p_1}\dotsm\|f_n\|_{p_n}.
    \]
  \item Use part (a) to show that that if \(1\leq p,q,r\leq\infty\), with
    \(1/p+1/q=1/r+1\), \(f\in L^p(\bbR)\), and \(g\in L^q(\bbR)\), then
    \[
      |(f*g)(x)|^r\leq{\|f\|_p}^{\cramped r-p}{\|g\|_q}^{\cramped r-q}\int|f(y)|^p|g(x-y)|^q\diff
      y.
    \]
    \\\\
    (Recall that \((f*g)(x)=\int f(y)g(x-y)\diff y\).)
  \item Prove \emph{Young's convolution theorem}: Assume that \(p\), \(q\),
    \(r\), \(f\), and \(g\) are as in part (b). Then \(f*g\in L^r(\bbR)\)
    and
    \[
      \|f*g\|_r\leq\|f\|_p\|g\|_q.
    \]
  \end{enumerate}
\end{problem}
\begin{solution}
  For (a) we shall proceed by induction on \(n\) the number of measurable
  functions \(f_j\in L^{p_j}(E)\), \(1\leq j\leq n\). The case \(n=2\)
  holds by using Hölder's inequality on the exponents \(r/p+r/q=1\),
  \begin{align*}
    \biggl[\int_E|f_1f_2|^r\biggr]^{1/r}\rmd x
    &=\|{f_1}^{\cramped{r}}{f_2}^{\cramped{r}}\|_1\\
    &\leq\|{f_1}^{\cramped r}\|_{p/r}\|{f_2}^{\cramped r}\|_{q/r}\\
    &=\|f_1\|_p\|f_2\|_q.
  \end{align*}
  Now, suppose this holds for \(n-1\) measurable functions
  \(f_j\in L^{p_j}(E)\), \(1\leq j\leq n-1\). Then for
  \(f_j\in L^{p_j}(E)\) with \(\sum_{j=1}^n 1/p_j=1/r\), we have
  \(r'=\sum_{j=1}^{n-1}1/p_j=1/r-1/p_n\) so by the inductive step
  \[
    \|f_1\dotsm f_{n-1}\|_{r'}\leq%
    \|f_1\|_{p_1}\dotsm\|f_{n-1}\|_{p_{n-1}}
  \]
  hence, \(f_1\dotsm f_{n-1}\in L^{r'}(E)\). Thus,
  \begin{align*}
    \|f_1\dotsm f_{n-1}f_n\|_r
    &\leq \|f_1\dotsm f_{n-1}\|_{r'}\|f_n\|_{p_n}\\
    &\leq\|f_1\|_{p_1}\dotsm\|f_{n-1}\|_{p_{n-1}}\|f_n\|_{p_n},
  \end{align*}
  as we set out to show.

  For part (b), applying the generalized Hölder's inequality we proved in
  part (a),
  \begin{align*}
    |f*g|
    &=\biggl|\int_\bbR f(y)g(x-y)\diff y\biggr|\\
    &\leq\int_\bbR\bigl|f(y)g(x-y)\bigr|\diff y\\
    &=\int_\bbR|f(y)|^{1+p/r-p/r}|g(x-y)|^{1+q/r-q/r}\diff y\\
    &=\int_\bbR|f(y)|^{p/r}|g(x)|^{q/r}|f(y)|^{1-p/r}|g(x-y)|^{1-q/r}\diff
      y\\
    &=\int_\bbR|f(y)|^{p/r}|g(x)|^{q/r}|f(y)|^{(r-p)/r}|g(x-y)|^{(r-q)/r}\diff
      y\\
    &=\int_\bbR\bigl(|f(y)|^p|g(x)|^q\bigr)^{1/r}|f(y)|^{(r-p)/r}
      |g(x-y)|^{(r-q)/r}\diff y\\
    &\leq
      \bigl\|\bigl(|f(y)|^p|g(x)|^q\bigr)^{1/r}\bigr\|_r
      \bigl\||f(y)|^{(r-p)/r}\bigr\|_{pr/(r-p)}
      \bigl\||g(x-y)|^{(r-q)/r}\bigr\|_{qr/(r-q)}\\
    &={\|f\|_p}^{\cramped{(r-p)/r}}{\|g\|_q}^{\cramped{(r-q)/r}}
      \biggl[\int_\bbR|f(y)|^p|g(x-y)|^q\diff y\biggr]^{1/r}.
  \end{align*}
  Raising both sides to the power \(r\), we have
  \[
    |(f*g)(x)|^r\leq{\|f\|_p}^{\cramped{r-p}}{\|g\|_q}^{\cramped{r-q}}\int|f(y)|^p|g(x-y)|^q\diff
    y,
  \]
  as desired.

  For part (c), using the estimate we worked out in part (b) together with
  Tonelli's theorem, we have
  \begin{align*}
    {\|f*g\|_r}^{\cramped{r}}
    &=\int_\bbR|f*g(x)|^r\diff x\\
    &\leq\int_\bbR
      \biggl[
      {\|f\|_p}^{\cramped{r-p}}{\|g\|_q}^{\cramped{r-q}}
      \int_\bbR|f(y)|^p|g(x-y)|^q\diff y
      \biggr]\\
    &={\|f\|_p}^{\cramped{r-p}}{\|g\|_q}^{\cramped{r-q}}
      \iint\limits_{\bbR\times\bbR}|f(y)|^p|g(x-y)|^q\diff
      y\\
    &={\|f\|_p}^{\cramped{r-p}}{\|g\|_q}^{\cramped{r-q}}
      \int_\bbR|f(y)|^p\biggl[\int_\bbR
      |g(x-y)|^q\diff y\biggr]\rmd x\\
    &\leq{\|f\|_p}^{\cramped r-p}{\|g\|_q}^{\cramped{r-q}}
      {\|f\|_p}^{\cramped{p}}{\|g_q\|}^{\cramped{q}}\\
    &={\|f\|_p}^{\cramped{r}}{\|g\|_q}^{\cramped{r}}.
  \end{align*}
  Taking the \(r\)th root on each side, we achieve the desired estimate
  \[
    \|f*g\|_r\leq \|f\|_p\|g\|_q.
  \]
\end{solution}

%%% Local Variables:
%%% mode: latex
%%% TeX-master: "../MA544-Quals"
%%% End:
