\begin{problem}
  Show that the function
  \[
    u(x,t)\defeq\sum_{k=-\infty}^\infty (-1)^k\Phi(x-2k,t)
  \]
  where
  \[
    \Phi(x,t)=\frac{\rme^{-\frac{x^2}{4t}}}{\sqrt{4\pi t}}
  \]
  is positive for \(|x|<1\), \(t>0\).

  \noindent (\emph{Hint:} Show that \(u\) satisfies \(u_t=u_{xx}\) for
  \(t>0\),
  \[
    \left\{
      \begin{aligned}
        u&=0&&\text{on \(\{\,|x|=1\,\}\times\{\,t\geq 0\,\}\),}\\
        u&=\delta_0&&\text{on \(\{\,|x|=1\,\}\times\{\,t=0\,\}\).}
      \end{aligned}
    \right.
  \]
  Then, carefully apply the maximum/minimum principle in a domain
  \(\{\,|x|\leq 1\,\}\times\{\,\varepsilon\leq t\leq T\,\}\) for small
  \(\varepsilon>0\) and large \(T>0\) pass to the limit as \(\varepsilon\to
  0^+\) and \(T\to\infty\).)
\end{problem}
\begin{solution}
  Taking the hint, let us verify that \(u_t=u_{xx}\), for \(t>0\). By
  direct computation, we have
  \begin{align*}
    \Phi_x(x,t)
    &=\frac{\partial}{\partial x}
      \left(\frac{\rme^{-\frac{x^2}{4t}}}{\sqrt{4\pi t}}\right)
    &\Phi_{xx}(x,t)
    &=\frac{\partial}{\partial x}
      \left(-\frac{x\rme^{-\frac{x^2}{4t}}}{2\sqrt{4\pi}t^{\frac{3}{2}}}\right)\\
    &=-\frac{x\rme^{-\frac{x^2}{4t}}}{2\sqrt{4\pi}t^{\frac{3}{2}}},
    &&=\frac{x^2\rme^{-\frac{x^2}{4t}}}{4\sqrt{4\pi}t^{\frac{5}{2}}}
      -\frac{\rme^{-\frac{x^2}{4t}}}{2\sqrt{4\pi}t^{\frac{3}{2}}}
    \\
    &&&=\frac{(x^2-2t)\rme^{-\frac{x^2}{4t}}}{4\sqrt{4\pi}t^{\frac{5}{2}}},
  \end{align*}
  and
  \begin{align*}
    \Phi_t(x,t)
    &=\frac{\partial}{\partial t}
      \left(\frac{\rme^{-\frac{x^2}{4t}}}{\sqrt{4\pi t}}\right)\\
    &=\frac{x^2\rme^{-\frac{x^2}{4t}}}{4\sqrt{4\pi}t^{\frac{5}{2}}}
      -\frac{\rme^{-\frac{x^2}{4t}}}{2\sqrt{4\pi}t^{\frac{3}{2}}}\\
    &=\frac{(x^2-2t)\rme^{-\frac{x^2}{4t}}}{4\sqrt{4\pi}t^{\frac{5}{2}}}.
  \end{align*}
  Since \(\Phi_t=\Phi_{xx}\) it follows that \(u_t=u_{xx}\) (for \(t>0\)).

  Next we show that \(u=0\) on \(\{\,|x|=1\,\}\times\{\,t\geq 0\,\}\) and
  \(u=\delta_0\) on \(\{\,|x|=1\,\}\times\{\,t=0\,\}\). To show \(u=0\) fix
  a \(t\geq 0\) and after relabeling, we may assume that \(x=1\) which
  gives us
  \begin{align*}
    u(1,t)
    &=\sum_{k=-\infty}^\infty(-1)^k\frac{\rme^{-\frac{k^2}{4t}}}{\sqrt{4\pi
      t}}\\
    &=\frac{1}{\sqrt{4\pi }t}\sum_{k=-\infty}^\infty
      (-1)^k{(\rme^{-\frac{1}{4t}})}^{k^2}\\
    &=
  \end{align*}
\end{solution}
\newpage

\begin{problem}[Tikhonov's example]
  Let
  \[
    g(t)\defeq
    \begin{cases}
      \rme^{-t^2}&t>0,\\
      0&t\leq 0.
    \end{cases}
  \]
  Then \(g\in C^\infty(\bfR)\) and we define
  \[
    u(x,t)\defeq\sum_{k=0}^\infty\frac{g^{(k)}(t)}{(2k)!}x^{2k}.
  \]
  Assuming that the series is convergent, show that \(u(x,t)\) solves the
  heat equation in \(\bfR\times(0,\infty)\) with the initial condition
  \(u(x,0)=0\), \(x\in\bfR\). Why doesn't this contradict the uniqueness
  theorem for the initial value problem?
\end{problem}
\begin{solution}
  Let \(u\) be as above. Then
  \begin{align*}
    u_t(x,t)
    &=\frac{\partial}{\partial t}
      \left(
      \sum_{k=0}^\infty\frac{g^{(k)}(t)}{(2k)!}x^{2k}
      \right)\\
    &=\sum_{k=0}^\infty \frac{g^{(k+1)}(t)}{(2k)!}x^{2k}\\
    &=\sum_{k=1}^\infty \frac{g^{(k)}(t)}{(2k-2)!}x^{2k-2},
  \end{align*}
  and
  \begin{align*}
    u_x(x,t)
    &=\frac{\partial}{\partial x}
      \left(
      \sum_{k=0}^\infty\frac{g^{(k)}(t)}{(2k)!}x^{2k}
      \right)
    &u_{xx}(x,t)
    &=\frac{\partial}{\partial x}
      \left(
      \sum_{k=0}^\infty\frac{g^{(k)}(t)}{(2k-1)!}x^{2k-1}
      \right)\\
    &=\sum_{k=0}^\infty\frac{g^{(k)}(t)}{(2k)!} 2kx^{2k-1}
    &&=\sum_{k=1}^\infty \frac{g^{(k)}(t)}{(2k-1)!}(2k-1)x^{2k-2}
       +\tfrac{\partial}{\partial x}g^{(0)}(t)\\
    &=\sum_{k=1}^\infty\frac{g^{(k)}(t)}{(2k-1)!}x^{2k-1},
    &&=\sum_{k=1}^\infty\frac{g^{(k)}(t)}{(2k-2)!}x^{2k-2}.
  \end{align*}
  Thus, \(u_t-\Delta u=0\); i.e., \(u\) solves the heat equation.
\end{solution}
\newpage

\begin{problem}
  Evaluate the integral
  \[
    \int_{-\infty}^\infty \cos(ax)\rme^{-x^2}\diff x,\qquad (a>0).
  \]
  \noindent (\emph{Hint:} Use the separation of variables to find the
  solution of the corresponding initial-value problem for the heat
  equation.)
\end{problem}
\begin{solution}
\end{solution}

%%% Local Variables:
%%% mode: latex
%%% TeX-master: "../MA523-HW-Current"
%%% End:
