\subsection{Homework 7}
\begin{problem}
  Solve the Dirichlet problem for the Laplace equation in \(\bbR^2\)
  \[
    \left\{
      \begin{aligned}
        \Lap u&=0&&\text{in \(1<|x|<2\),}\\
        u&=x_1&&\text{on \(|x|=1\),}\\
        u&=1+x_1x_2&&\text{on \(|x|=2\).}
      \end{aligned}
    \right.
  \]
  \\\\
  \emph{Hint:} Use Laurent series.
\end{problem}
\begin{solution*}
  First, let us make the change of variables \((x_1,x_2)\mapsto
  r\rme^{\rmi\theta}\) to the Dirichlet problem in question:
  \begin{equation}
    \label{eq:7:dirichlet-problem-polar}
    \left\{
      \begin{aligned}
        \Lap u&=0&&\text{in \(1<r<2\),}\\
        u&=\tfrac{1}{2}(\rme^{\rmi\theta}+\rme^{-\rmi\theta})&&\text{on \(r=1\),}\\
        u&=1+\tfrac{1}{i}(\rme^{\rmi 2\theta}-\rme^{-\rmi 2\theta})&&\text{on \(r=2\).}
      \end{aligned}
    \right.
  \end{equation}

  Now, suppose \(u\) is a solution, of the form
  \[
    u(r\rme^{\rmi\theta})=%
    b\ln r%
    +\sum_{n=-\infty}^\infty (a_nr^n+\overline{a_{-n}}r^{-n})\rme^{\rmi n\theta},
  \]
  to the problem \eqref{eq:7:dirichlet-problem-polar}. It is easy to see
  that \(u\) is in fact harmonic:
  \begin{align*}
    \Lap u%
    &=u_{rr}+\tfrac{1}{r}u_r+\tfrac{1}{r^2}u_{\theta\theta}\\
    &=-br^{-2}+br^{-2}+\sum_{n=-\infty}^\infty
      \left[\bigl(n(n-1)+n-n^2\bigr) a_nr^n\right.\\
    &\phantom{{}={}-\frac{b}{r^2}+\frac{b}{r^2}+}
      \left.+\bigl(n(n-1)+n-n^2\bigr)\overline{a_{-n}}r^{-n}\right]\rme^{\rmi
      n\theta}\\
    &=0.
  \end{align*}

  Next we use the boundary data to compute the coefficients \(a_n\),
  \(n\in\bfZ\). Using the data \eqref{eq:7:dirichlet-problem-polar}, on
  \(r=1\) we have
  \[
    \tfrac{1}{2}(\rme^{\rmi\theta}+\rme^{-\rmi\theta})%
    =\sum_{n=-\infty}^\infty (a_n+\overline{a_{-n}})\rme^{\rmi n\theta},
  \]
  and on \(r=2\)
  \[
    1+\tfrac{1}{i}(\rme^{\rmi 2\theta}-\rme^{-\rmi 2\theta}) = b\ln
    2+\sum_{n=-\infty}^\infty (2^na_n+2^{-n}a_{-n})\rme^{\rmi n\theta}.
  \]
  These equations immediately tell us that \(b=1/{\ln 2}\). Moreover, the
  following relations on the coefficients hold
  \[
    \left\{
    \begin{aligned}
      \frac{1}{2}&=a_1+\overline{a_{-1}}
      &\frac{1}{2}&=a_{-1}+\overline{a_1},\\
      \frac{1}{i}&=2^2a_2+2^{-2}\overline{a_{-2}},
      &-\frac{1}{i}&=2^2a_{-2}+2^{-2}\overline{a_{2}},\\
      0&=a_n+\overline{a_{-n}}&&&&\text{for \(n\neq\pm 1\),}\\
      0&=2^{n}a_n+2^{-n}\overline{a_{-n}}&&&&\text{for \(n\neq\pm 2\).}
    \end{aligned}
    \right.
  \]
  A little calculation shows that
  \[
    \left\{
      \begin{aligned}
        a_1&=-\frac{1}{6},&a_{-1}&=\frac{2}{3},\\
        a_2&=-\frac{4\rmi}{15},&a_{-2}&=-\frac{4\rmi}{15},\\
        a_n&=0&&&&\text{for \(n\neq \pm 1,\pm 2\).}
      \end{aligned}
    \right.
  \]
  Thus,
  \[
    \begin{aligned}
      u(r\rme^{\rmi\theta})
      &=\tfrac{1}{\ln 2}\ln r
      +\left(-\tfrac{4\rmi}{15}r^{-2}+\tfrac{4\rmi}{15}r^2\right)\rme^{-\rmi
        2\theta} +\left(\tfrac{2}{3}r^{-1}-\tfrac{1}{6}r\right)\rme^{-\rmi\theta}\\
      &\phantom{{}={}}
      +\left(-\tfrac{1}{6}r+\tfrac{2}{3}r^{-1}\right)\rme^{\rmi\theta}
      +\left(-\tfrac{4\rmi}{15}r^2+\tfrac{4\rmi}{15}r^{-2}\right)\rme^{\rmi
        2\theta}\\
      &=\tfrac{1}{\ln 2}\ln r-\tfrac{8}{15}r^{-4}
      \left(\frac{r^2\rme^{\rmi 2\theta}-r^2\rme^{-\rmi 2\theta}}{2\rmi}\right)
      +\tfrac{8}{15}
      \left(\frac{r^2\rme^{\rmi 2\theta}-r^2\rme^{-\rmi
            2\theta}}{2\rmi}\right)\\
      &\phantom{{}={}}
      +\tfrac{4}{3}r^{-2}
      \left(\frac{r\rme^{\rmi\theta}+r\rme^{-\rmi\theta}}{2}\right)
      -\tfrac{1}{3}
      \left(\frac{r\rme^{\rmi\theta}+r\rme^{-\rmi\theta}}{2}\right).
    \end{aligned}
  \]
  Substituting back, we have
  \begin{equation}
    \label{eq:7:solution-to-dirichlet-problem}
    u(x_1,x_2)=\tfrac{1}{\ln 2}\ln(x_1^2+x_2^2)
    -\frac{16x_1x_2}{15{(x_1^2+x_2^2)}^2}+\frac{16x_1x_2}{15}
    +\frac{4x_1}{3(x_1^2+x_2^2)}-\frac{x_1}{3}.
  \end{equation}
  It is easy to see that \eqref{eq:7:solution-to-dirichlet-problem}
  satisfies the boundary data at \(|x|=1\) and \(|x|=2\).
\end{solution*}

\begin{problem}
  Let \(\Omega\) be a bounded domain with a \(C^1\) boundary, \(g\in
  C^2(\partial\Omega)\) and \(f\in C(\bar\Omega)\). Consider the so called
  \emph{Neumann problem}
  \[
    \label{eq:7:neumann-problem}%
    \tag{\(*\)}%
    \left\{
      \begin{aligned}
        -\Lap u&=f&&\text{in \(\Omega\),}\\
        \frac{\partial u}{\partial\nu}&=g&&\text{on \(\partial\Omega\),}
      \end{aligned}
    \right.
  \]
  where \(\nu\) is the outer normal on \(\partial\Omega\). Show that the
  solution of \eqref{eq:7:neumann-problem} in
  \(C^2(\Omega)\cap C^1(\bar\Omega)\) is unique up to a constant; i.e., if
  \(u_1\) and \(u_2\) are both solutions of \eqref{eq:7:neumann-problem},
  then \(u_2=u_1+\text{const.}\)\@ in \(\Omega\).
  \\\\
  \emph{Hint:} Look at the proof of the uniqueness for the Dirichlet
  problem by energy methods [E, 2.2.5a].
\end{problem}
\begin{solution*}
  Suppose \(u_1\) and \(u_2\) are solutions to the Neumann problem
  \eqref{eq:7:neumann-problem}. Define \(v\defeq u_1-u_2\). Then \(v\) is
  harmonic in \(\Omega\) and \(\partial v/\partial \nu=0\) on
  \(\partial\Omega\). Consider the energy functional
  \[
    E[v]=\frac{1}{2}\int_\Omega|Dv|^2\diff x.
  \]
  By Green's formula version (ii),
  \begin{align*}
    E[v]
    &=\frac{1}{2}\int_\Omega|Dv|^2\diff x\\
    &=-\frac{1}{2}\int_\Omega v\Lap v\diff x
      +\int_{\partial U}\frac{\partial
      v}{\partial\nu} v\diff S(x)\\
    &=0.
  \end{align*}
  This implies that \(|Dv|^2=Dv\cdot Dv=0\) which, since the standard inner
  product on \(\bbR^n\) is positive-definite, implies that \(Dw\equiv
  0\). It follows that \(u_1=u_2+\text{const}\), i.e., the solution \(u\)
  to \eqref{eq:7:neumann-problem} is unique up to a constant.
\end{solution*}

\begin{problem}
  Write down an explicit formula for a solution of
  \[
    \left\{
      \begin{aligned}
        u_t-\Lap_x u+cu&=f&&\text{in \(\bbR^n\times(0,\infty)\),}\\
        u&=g&&\text{on \(\bbR^n\times\{\,t=0\,\}\),}
      \end{aligned}
    \right.
  \]
  where \(c\in\bbR\).
  \\\\
  \emph{Hint:} Rewrite the problem in terms of
  \(v(x,t)\defeq\rme^{ct}u(x,t)\).
\end{problem}
\begin{solution*}
  Taking the hint, let us rewrite the problem in terms of
  \(v(x,t)=\rme^{ct}u(x,t)\):
  \begin{equation}
    \label{eq:7:heat-problem-exp}
    \left\{
      \begin{aligned}
        v_t-\Lap_xv&=\rme^{ct}f&&\text{in
          \(\bbR^n\times(0,\infty),\)}\\
        v&=g&&\text{on \(\bbR^n\times\{\,t=0\,\}\).}
      \end{aligned}
    \right.
  \end{equation}
  By Duhamel's principle, the problem \eqref{eq:7:heat-problem-exp} is
  solved by
  \[
    v(x,t)=\int_{\bbR^n}\Phi(x-y,t)g(y)\diff y
    +\int_0^t\int_{\bbR^n}\Phi(x-y,t-s)\rme^{cs}f(y,s)\diff yds,
  \]
  where \(\Phi\) is the fundamental solution to the heat equation. Thus,
  the formula
  \[
    u(x,t)=\rme^{-ct}v(x,t)=\rme^{-ct}\int_{\bbR^n}\Phi(x-y,t)g(y)\diff y
    +\rme^{-ct}\int_0^t\int_{\bbR^n}\Phi(x-y,t-s)\rme^{cs}f(y,s)\diff yds
  \]
  solves the original problem.
\end{solution*}

%%% Local Variables:
%%% mode: latex
%%% TeX-master: "../MA523-HW-ALL"
%%% End:
